src/Narcissus/Examples/NetworkStack/bench.ml
@@ -3,10 +3,12 @@ open Fiat4Mirage
 
 let () =
   Core.Command.run (Bench.make_command [
-    Bench.Test.create ~name:"id"
-      (fun () -> ());
+    (* Bench.Test.create ~name:"id"
+     *   (fun () -> ()); *)
     (* Bench.Test.create ~name:"packet_iter"
      *   (fun () -> ignore (Array.fold_left (fun acc x -> acc + 1) 0 bin_pkt)); *)
     Bench.Test.create ~name:"fiat_ipv4_decode"
       (fun () -> ignore (fiat_ipv4_decode_bench ()));
+    Bench.Test.create ~name:"fiat_ipv4_encode"
+      (fun () -> ignore (fiat_ipv4_encode_bench ()));
   ])
