src/Narcissus/Examples/NetworkStack/bench.sh
@@ -1,4 +1,4 @@
 #!/usr/bin/env sh
 ocamlopt -config
-ocamlfind ocamlopt -linkpkg -thread -package core -package core_bench ArrayVector.ml Fiat4Mirage.mli Fiat4Mirage.ml bench.ml -o fiat4mirage-bench || exit 1
+ocamlfind ocamlopt -linkpkg -thread -package core -package core_bench Int64Word.ml ArrayVector.ml Fiat4Mirage.mli Fiat4Mirage.ml bench.ml -o fiat4mirage-bench || exit 1
 ./fiat4mirage-bench
